src/proof/hashtriemap/model.v
@@ -53,12 +53,14 @@ Section model.
     [∗ list] hash ∈ dom, ptsto_mut γ hash q (f hash).
 
   Global Opaque own_domain.
+  Local Transparent own_domain.
 
   Definition own_path
     (γ : gname) (q: Qp) (p : path) (f: Z → gmap K V) : iProp Σ :=
     own_domain γ q (path_to_domain p) f.
 
   Global Opaque own_path.
+  Local Transparent own_path.
 
   (* Constant function: all hashes map to empty *)
   Definition empty_map_fn : Z → gmap K V := λ _, ∅.
@@ -70,7 +72,315 @@ Section model.
   Definition flatten (hm: hash_map) : gmap K V :=
     map_fold (λ (_: Z) (sub: gmap K V) (acc: gmap K V), sub ∪ acc) ∅ hm.
 
-  Lemma own_path_lookup γ q path h f :
+  #[global] Instance own_path_timeless γ dom q f : Timeless (own_path γ q dom f) := _.
+
+  #[global] Instance own_path_fractional γ dom f :
+    Fractional (λ q, own_path γ q dom f).
+  Proof.
+    intros p q. rewrite /own_path /own_domain -big_sepL_sep.
+    iSplit.
+    - iIntros "H1".
+      iApply (big_sepL_mono with "H1").
+      iIntros (i h Hin) "Hh1".
+      iDestruct "Hh1" as "[Hh1 Hh2]".
+      iFrame.
+    - iIntros "H1".
+      iApply (big_sepL_mono with "H1").
+      iIntros (i h Hin) "Hh1".
+      iDestruct "Hh1" as "[Hh1 Hh2]".
+      iCombine "Hh1 Hh2" as "Hh".
+      iFrame.
+  Qed.
+
+  #[global] Instance own_path_as_fractional γ path f q :
+    AsFractional (own_path γ q path f) (λ q, own_path γ q path f) q.
+  Proof.
+    split; [done|apply _].
+  Qed.
+
+  Definition entry_inv
+    (γ: ghost_names) (q: Qp)
+    (entry: loc -d> path -d> iProp Σ)
+    (e: loc) (path: path) : iProp Σ :=
+    (if decide (e = null) then
+       own_path γ.(map_name) q path empty_map_fn
+     else
+       ∃ (next: loc) (k: K) (v: V) (h: Z) rest_map,
+         "#Hk" :: e ↦s[hashtriemap.entry :: "key"]□ k ∗
+         "#Hv" :: e ↦s[hashtriemap.entry :: "value"]□ v ∗
+         "%Hhash" :: ⌜uint.Z (hash_key k) = h⌝ ∗
+         "%Hbelongs" :: ⌜belongs_to_path path h⌝ ∗
+         "Hown_next" :: (struct.field_ref_f hashtriemap.entry "overflow" e) ↦ᵥ{q} (interface.mk (ptrT.id hashtriemap.entry.id) #next) ∗
+         "Hown_path" :: own_path γ.(map_name) q path (singleton_map_fn h (<[k:=v]> rest_map)) ∗
+         if decide (next = null) then
+           ⌜rest_map = ∅⌝
+         else
+           "#Hnext_entry" :: ▷ entry next path)%I.
+
+  Definition entry_F
+    (γ: ghost_names) (q: Qp)
+    (entry: loc -d> path -d> iProp Σ)
+    : loc -d> path -d> iProp Σ :=
+    λ e path,
+      ("#Hentry_inv" :: inv entryN (entry_inv γ q entry e path))%I.
+
+  Global Instance entry_F_contractive γ q : Contractive (entry_F γ q).
+  Proof.
+    rewrite /entry_F /entry_inv.
+    intros n f g Hfg e path.
+    f_equiv.
+    f_equiv.
+    f_equiv.
+    f_equiv.
+    f_equiv.
+    f_equiv.
+    f_equiv.
+    solve_contractive.
+  Qed.
+
+  Definition entry (γ: ghost_names) (q: Qp) (e: loc) (path: path) : iProp Σ :=
+    fixpoint (entry_F γ q) e path.
+
+  Lemma entry_unfold γ q e path :
+    entry γ q e path ⊣⊢ entry_F γ q (entry γ q) e path.
+  Proof. apply (fixpoint_unfold (entry_F γ q)). Qed.
+
+  #[global] Instance entry_persistent γ q e path : Persistent (entry γ q e path).
+  Proof.
+    rewrite entry_unfold /entry_F.
+    apply _.
+  Qed.
+
+  Definition childP
+    (child_indirect: loc -d> path -d> iProp Σ)
+    (γ: ghost_names) (q: Qp)
+    nodeptr (path child_path: path) : iProp Σ :=
+    if (decide (nodeptr = null)) then
+      own_path γ.(map_name) q path empty_map_fn
+    else
+      (∃ (is_entry: bool),
+          nodeptr ↦s[hashtriemap.node :: "isEntry"]□ is_entry ∗
+          if is_entry then
+            ∃ ent,
+              ⌜ent ≠ null⌝ ∗
+              nodeptr ↦s[hashtriemap.node :: "ent"]□ ent ∗
+              nodeptr ↦s[hashtriemap.node :: "ind"]□ null ∗
+              entry γ q ent path
+          else
+            ∃ ind,
+              ⌜length child_path < 16⌝ ∗
+              nodeptr ↦s[hashtriemap.node :: "ent"]□ null ∗
+              nodeptr ↦s[hashtriemap.node :: "ind"]□ ind ∗
+              ▷ child_indirect ind child_path)%I.
+
+  Definition childrenP
+    (child_indirect: loc -d> path -d> iProp Σ)
+    (γ: ghost_names) (q: Qp) (children_slice: slice.t)
+    (children_vals: list atomic.Value.t)
+    (ind: loc) (path: path) : iProp Σ :=
+    "Hchildren" :: [∗ list] i ↦ val ∈ children_vals,
+      let child_path := path ++ [Z.of_nat i] in
+      ∃ (nodeptr: loc),
+        "Hown_child" :: own_Value (slice.elem_ref_f children_slice atomic.Value i) (DfracOwn q)
+          (interface.mk (ptrT.id hashtriemap.node.id) #nodeptr) ∗
+        "Hchild" :: childP child_indirect γ q nodeptr path child_path.
+
+  (* split 50/50 between an invariant and the mutex to allow for lock-free reads *)
+  (* we always have read permission on any indirect, but only can write if we acquire the lock *)
+  (* the only things ever modified are atomic values (atomic pointers), everything else is □ ownership *)
+  Definition indirect_F
+    (γ: ghost_names)
+    (indirect: loc -d> (list Z) -d> iProp Σ)
+    : loc -d> (list Z) -d> iProp Σ :=
+    λ ind path,
+      (∃ (children_vals: list atomic.Value.t) children_slice,
+          "#Hown_children" :: ind ↦s[hashtriemap.indirect :: "children"]□ children_slice ∗
+          "#Hchildren_slice" :: children_slice ↦*□ children_vals ∗
+          "%Hchildren_len" :: ⌜length children_vals = 16%nat⌝ ∗
+          (* "#Hmutex" :: ind ↦s[hashtriemap.indirect :: "mu"]□ mutex ∗ *)
+          "#Hind_inv" :: inv (indN) ((childrenP indirect γ (1/2) children_slice children_vals ind path)) ∗
+          "#Hind_mutex" :: is_Mutex (struct.field_ref_f hashtriemap.indirect "mu" ind) (
+              ∃ (dead: bool),
+                "Hdead" ∷ own_Bool (struct.field_ref_f hashtriemap.indirect "dead" ind) (DfracOwn 1) dead ∗
+                "Hmu_inv" ∷ ((* ⌜¬ dead⌝ -∗  *)childrenP indirect γ (1/2) children_slice children_vals ind path)))%I.
+
+  (* Prove contractiveness *)
+  Global Instance indirect_F_contractive γ : Contractive (indirect_F γ).
+  Proof.
+    rewrite /indirect_F.
+    intros n f g Hfg ind path.
+    f_equiv.
+    f_equiv.
+    f_equiv.
+    f_equiv.
+    have H : ((childrenP f γ (1 / 2) a0 a ind path) ≡{n}≡ (childrenP g γ (1 / 2) a0 a ind path)).
+    { unfold childrenP. repeat f_equiv. unfold childP. solve_contractive. }
+    repeat f_equiv; exact H.
+  Qed.
+
+  Definition indirect (γ: ghost_names) (ind: loc) (path: path) : iProp Σ :=
+    fixpoint (indirect_F γ) ind path.
+
+  Lemma indirect_unfold γ ind path :
+    indirect γ ind path ⊣⊢
+    indirect_F γ (indirect γ) ind path.
+  Proof. apply (fixpoint_unfold (indirect_F γ)). Qed.
+
+  #[global] Instance indirect_persistent γ ind path : Persistent (indirect γ ind path).
+  Proof.
+    rewrite indirect_unfold /indirect_F.
+    apply _.
+  Qed.
+
+  (* Abstract map state seen by clients. *)
+  Definition own_ht_map (γ: ghost_names) (m: gmap K V) : iProp Σ :=
+    ghost_var γ.(user_name) (DfracOwn (1/2)) m.
+
+  Definition map_state (γ: ghost_names) (user_map: gmap K V) (hm: hash_map) : iProp Σ :=
+    "Hauth_map" :: map_ctx γ.(map_name) 1 hm ∗
+    "Huser_map" :: ghost_var γ.(user_name) (DfracOwn (1/2)) user_map ∗
+    "%Hflat" :: ⌜user_map = flatten hm⌝ ∗
+    (* bucket correctness - if a key exists, then its in the correct bucket *)
+    "%Hbuckets" :: (⌜∀ h sub k, hm !! h = Some sub →
+                               uint.Z (hash_key k) = h →
+                               flatten hm !! k = sub !! k⌝) ∗
+    "%Hbuckets_rev" ∷ (⌜∀ h sub k v,
+                         hm !! h = Some sub →
+                         sub !! k = Some v →
+                         uint.Z (hash_key k) = h⌝).
+
+  Definition own_root
+    (γ: ghost_names) (ht: loc) (rooti: loc) : iProp Σ :=
+    "Hown_root" ∷ (struct.field_ref_f hashtriemap.HashTrieMap "root" ht) ↦ᵥ
+      (interface.mk (ptrT.id hashtriemap.indirect.id) #rooti) ∗
+    "#Hroot_indirect" ∷ indirect γ rooti [].
+
+  Definition ht_inv
+    (γ: ghost_names) (ht: loc) : iProp Σ :=
+    inv mapN (
+        "Hroot" ∷ (∃ root, "Hroot" ∷ own_root γ ht root) ∗
+        "Hmap" ∷ (∃ user_map hm, "Hmap" ∷ map_state γ user_map hm)
+      ).
+
+  (* Public predicate exposed to clients. *)
+  Definition is_hashtriemap
+    (γ: ghost_names) (ht: loc) : iProp Σ :=
+    ("#Hseed" :: ∃ (seed: w64), ht ↦s[hashtriemap.HashTrieMap :: "seed"]□ seed) ∗
+    "#His_map" :: ht_inv γ ht.
+
+  Definition ht_au_mask : coPset :=
+    ⊤ ∖ ↑mapN ∖ ↑indN ∖ ↑entryN.
+
+  (* Helper for Load return values. *)
+  Definition ht_load_ret (m: gmap K V) (key: K) : val :=
+    (match m !! key with
+    | Some v => (#v, #true)
+    | None => (#(default_val V), #false)
+    end)%V.
+
+  (* designed to be split between an invariant and a mutex, so that reading can be done outside of the critical section and writing can only be done inside *)
+  Definition init_tok `{!ghost_varG Σ bool} (γ: ghost_names) (b: bool) : iProp Σ :=
+    ghost_var γ.(init_name) (DfracOwn (1/2)) b.
+
+  Definition init_status_done
+    (γ: ghost_names) (ht: loc) (b: bool) : iProp Σ :=
+    (if b then is_hashtriemap γ ht else True%I).
+
+  Definition init_status_inv
+    `{!ghost_varG Σ bool}
+    (ht: loc) (γ: ghost_names) : iProp Σ :=
+    ∃ (b: bool),
+      own_Uint32 (struct.field_ref_f hashtriemap.HashTrieMap "inited" ht) 1
+        (if b then W32 1 else W32 0) ∗
+      init_tok γ b ∗
+      □ init_status_done γ ht b.
+
+  Definition init_status
+    `{!ghost_varG Σ bool}
+    (ht: loc) (γ: ghost_names) : iProp Σ :=
+    inv init_statusN (init_status_inv ht γ).
+
+  (* Initialization lock invariant for HashTrieMap. *)
+  Definition init_mu_inv `{!ghost_varG Σ bool}
+    (ht: loc) (γ: ghost_names) : iProp Σ :=
+    ∃ (b: bool),
+      if b
+      then init_tok γ true
+      else (init_tok γ false ∗
+            (∃ (seed: w64),
+                ht ↦s[hashtriemap.HashTrieMap :: "seed"] seed) ∗
+            own_Value (struct.field_ref_f hashtriemap.HashTrieMap "root" ht) 1 interface.nil
+           )%I.
+
+  Definition init_mu `{!ghost_varG Σ bool}
+    (ht: loc) (γ: ghost_names) : iProp Σ :=
+    is_Mutex (struct.field_ref_f hashtriemap.HashTrieMap "initMu" ht)
+      (init_mu_inv ht γ).
+
+  Definition hashtriemap_init
+    `{!ghost_varG Σ bool}
+    (ht: loc) (γ: ghost_names) : iProp Σ :=
+    "#Hinit" :: init_status ht γ ∗
+    "#Hinit_mu" :: init_mu ht γ.
+
+  Lemma hashtriemap_pre_auth_init
+    `{!mapG Σ w64 w64, !ghost_varG Σ (gmap w64 w64), !ghost_varG Σ bool} :
+    ⊢ |==> ∃ γ,
+      init_tok γ false ∗ init_tok γ false.
+  Proof.
+    iMod (ghost_var_alloc (false)) as (init_γ) "[Hinit1 Hinit2]".
+    iMod (ghost_var_alloc (∅ : gmap K V)) as (map_γ) "Hmap".
+    iMod (ghost_var_alloc (∅ : gmap K V)) as (user_γ) "[Huser1 Huser2]".
+    iModIntro.
+    iExists (mkNames map_γ init_γ user_γ).
+    iFrame.
+  Qed.
+
+  Lemma hashtriemap_zero_init
+    `{!mapG Σ Z (gmap K V), !mapG Σ K V, !ghost_varG Σ (gmap w64 w64), !ghost_varG Σ bool}
+    (ht: loc) E (P: gmap w64 w64 → iProp Σ) :
+    ht ↦ default_val hashtriemap.HashTrieMap.t ={E}=∗
+    ∃ γ, hashtriemap_init ht γ.
+  Proof.
+    iIntros "Hht".
+    iDestruct (struct_fields_split with "Hht") as "Hfields".
+    iNamed "Hfields".
+    simpl.
+    iMod (hashtriemap_pre_auth_init) as (γ) "(Htok1 & Htok2)".
+
+    iApply struct_fields_split in "Hinited".
+    iNamed "Hinited".
+    iDestruct (Uint32_unfold with "Hv") as "Hinited".
+    iClear "H_0".
+
+    iApply struct_fields_split in "Hroot".
+    iNamed "Hroot".
+    simpl.
+    iDestruct (Value_unfold with "Hv") as "Hroot".
+
+    iMod (inv_alloc init_statusN _ (init_status_inv ht γ) with "[Htok1 Hinited]") as "#Hinit".
+    {
+      iNext.
+      iExists false.
+      iFrame.
+      done.
+    }
+    set (m := struct.field_ref_f hashtriemap.HashTrieMap "initMu" ht).
+
+    iMod (init_Mutex (init_mu_inv ht γ) E m with "HinitMu [Htok2 Hseed Hroot]") as "Hmutex".
+    {
+      iNext.
+      iExists false.
+      iFrame.
+    }
+
+    iModIntro.
+    iExists γ.
+    iFrame.
+    iFrame "#".
+  Qed.
+
+  Lemma own_path_lookup h path γ q f :
     h ∈ path_to_domain path →
     own_path γ q path f -∗
     ptsto_mut γ h q (f h) ∗ (ptsto_mut γ h q (f h) -∗ own_path γ q path f).
@@ -201,15 +511,6 @@ Section model.
       reflexivity.
   Qed.
 
-  Lemma dom_no_dup p : NoDup (path_to_domain p).
-  Proof.
-    unfold path_to_domain.
-    apply NoDup_filter.
-    Local Transparent full_domain.
-    unfold full_domain.
-    apply NoDup_seqZ.
-  Qed.
-
   Lemma own_path_update_key key value γ hm path f :
     let h  := uint.Z (hash_key key) in
     let f' := (λ h', if decide (h' = h) then <[key:=value]>(f h) else f h') in
@@ -228,27 +529,22 @@ Section model.
     have Hdom : h ∈ path_to_domain path
                   by apply (path_to_domain_elem _ _);
       [apply full_domain_elem|exact Hbelongs].
-    Local Transparent own_path.
-    unfold own_path.
+    unfold own_path, own_domain.
     set (dom := path_to_domain path) in *.
-    have Hnodup : NoDup dom.
-    { apply dom_no_dup. }
+    have Hnodup : NoDup dom by apply dom_no_dup.
     iInduction dom as [|h' dom] "IH".
     { rewrite elem_of_nil in Hdom. done. }
     apply NoDup_cons in Hnodup as [Hnotin Hnodup].
-    iSimpl in "Hpath".
+    simpl.
+    iDestruct "Hpath" as "[Hh Hpath]".
     rewrite elem_of_cons in Hdom.
-    Local Transparent own_domain.
-    iDestruct "Hpath" as "[Hh' Hpath]".
     destruct Hdom as [Heq | Hdom].
     - subst h'.
       (* h not in domain, so cant use IH *)
       iClear "IH".
-      iMod (map_update h (f h) (f' h) with "Hctx Hh'") as "[Hctx Hh]".
+      iMod (map_update h (f h) (f' h) with "Hctx Hh") as "[Hctx Hh]".
       iModIntro.
       iFrame "Hctx".
-      unfold own_domain.
-      rewrite big_sepL_cons.
       iFrame.
       subst f'.
       simpl.
@@ -259,396 +555,180 @@ Section model.
       subst.
       apply Hnotin.
       apply (list_elem_of_lookup_2 _ _ _ Hy).
-    - iAssert (⌜h ∈ dom⌝)%I as "Hdom'".
-      { iPureIntro. exact Hdom. }
-      iAssert (⌜NoDup dom⌝)%I as "Hnodup'".
-      { iPureIntro. exact Hnodup. }
-      repeat iSpecialize ("IH" with "[$]").
+    - iSpecialize ("IH" $! Hdom Hnodup with "Hctx Hpath").
       iMod "IH".
       iModIntro.
       iDestruct "IH" as "(Hctx & Hpath)".
       iFrame "Hctx".
-      unfold own_domain.
-      rewrite big_sepL_cons.
       iFrame.
       subst f'.
       simpl.
-      rewrite decide_False; [iFrame|].
-      intro Heq.
-      subst.
-      exact (Hnotin Hdom).
-  Qed.
-
-  #[global] Instance own_path_timeless γ dom q f : Timeless (own_path γ q dom f) := _.
-
-  #[global] Instance own_path_fractional γ dom f :
-    Fractional (λ q, own_path γ q dom f).
-  Proof.
-    intros p q. rewrite /own_path /own_domain -big_sepL_sep.
-    iSplit.
-    - iIntros "H1".
-      iApply (big_sepL_mono with "H1").
-      iIntros (i h Hin) "Hh1".
-      iDestruct "Hh1" as "[Hh1 Hh2]".
-      iFrame.
-    - iIntros "H1".
-      iApply (big_sepL_mono with "H1").
-      iIntros (i h Hin) "Hh1".
-      iDestruct "Hh1" as "[Hh1 Hh2]".
-      iCombine "Hh1 Hh2" as "Hh".
+      have Hneq : h' ≠ h by intros Heq; subst h'; exact (Hnotin Hdom).
+      rewrite (decide_False _ _ Hneq).
       iFrame.
   Qed.
 
-  #[global] Instance own_path_as_fractional γ path f q :
-    AsFractional (own_path γ q path f) (λ q, own_path γ q path f) q.
+  Lemma hm_lookup {h path γ m hm fn q} :
+    h ∈ path_to_domain path →
+    map_state γ m hm -∗
+    own_path γ.(map_name) q path fn -∗
+    ⌜hm !! h = Some (fn h)⌝.
   Proof.
-    split; [done|apply _].
+    iIntros (Hdom) "Hmap_state Hown_path".
+    iNamed "Hmap_state".
+    iDestruct (own_path_lookup h _ _ _ _ Hdom with "Hown_path") as "[Hptsto Hptsto_close]".
+    iDestruct (map_valid with "Hauth_map Hptsto") as %Hlookup.
+    done.
   Qed.
 
-  Definition entry_inv
-    (γ: ghost_names) (q: Qp)
-    (entry: loc -d> path -d> iProp Σ)
-    (e: loc) (path: path) : iProp Σ :=
-    (if decide (e = null) then
-       own_path γ.(map_name) q path empty_map_fn
-     else
-       ∃ (next: loc) (k: K) (v: V) (h: Z) rest_map,
-         "#Hk" :: e ↦s[hashtriemap.entry :: "key"]□ k ∗
-         "#Hv" :: e ↦s[hashtriemap.entry :: "value"]□ v ∗
-         "%Hhash" :: ⌜uint.Z (hash_key k) = h⌝ ∗
-         "%Hbelongs" :: ⌜belongs_to_path path h⌝ ∗
-         "Hown_next" :: own_Value (struct.field_ref_f hashtriemap.entry "overflow" e) (DfracOwn q) (interface.mk (ptrT.id hashtriemap.entry.id) #next) ∗
-         "Hown_path" :: own_path γ.(map_name) q path (singleton_map_fn h (<[k:=v]> rest_map)) ∗
-         if decide (next = null) then
-           ⌜rest_map = ∅⌝
-         else
-           "#Hnext_entry" :: ▷ entry next path)%I.
-
-  Definition entry_F
-    (γ: ghost_names) (q: Qp)
-    (entry: loc -d> path -d> iProp Σ)
-    : loc -d> path -d> iProp Σ :=
-    λ e path,
-      ("#Hentry_inv" :: inv entryN (entry_inv γ q entry e path))%I.
-
-  Global Instance entry_F_contractive γ q : Contractive (entry_F γ q).
+  Lemma user_map_lookup {h path γ m hm fn q k} :
+    h ∈ path_to_domain path →
+    h = uint.Z (hash_key k) →
+    map_state γ m hm -∗
+    own_path γ.(map_name) q path fn -∗
+    ⌜m !! k = (fn h) !! k⌝.
   Proof.
-    rewrite /entry_F /entry_inv.
-    intros n f g Hfg e path.
-    f_equiv.
-    f_equiv.
-    f_equiv.
-    f_equiv.
-    f_equiv.
-    f_equiv.
-    f_equiv.
-    solve_contractive.
+    iIntros (Hdom Hh) "Hmap_state Hown_path".
+    iDestruct (hm_lookup Hdom with "Hmap_state Hown_path") as %Hhm.
+    iNamed "Hmap_state".
+    rewrite Hflat.
+    iPureIntro.
+    apply (Hbuckets h (fn h) k); auto.
   Qed.
 
-  Definition entry (γ: ghost_names) (q: Qp) (e: loc) (path: path) : iProp Σ :=
-    fixpoint (entry_F γ q) e path.
-
-  Lemma entry_unfold γ q e path :
-    entry γ q e path ⊣⊢ entry_F γ q (entry γ q) e path.
-  Proof. apply (fixpoint_unfold (entry_F γ q)). Qed.
-
-  #[global] Instance entry_persistent γ q e path : Persistent (entry γ q e path).
+  Lemma map_state_agree {γ m m2 hm} :
+    map_state γ m hm -∗ own_ht_map γ m2 -∗ ⌜m = m2⌝.
   Proof.
-    rewrite entry_unfold /entry_F.
-    apply _.
+    iIntros "Hmap_state Huser_map2".
+    iNamed "Hmap_state".
+    iDestruct (ghost_var_agree with "Huser_map Huser_map2") as %Hx.
+    done.
   Qed.
 
-  Definition childP
-    (child_indirect: loc -d> path -d> iProp Σ)
-    (γ: ghost_names) (q: Qp)
-    nodeptr (path child_path: path) : iProp Σ :=
-    if (decide (nodeptr = null)) then
-      own_path γ.(map_name) q path empty_map_fn
-    else
-      (∃ (is_entry: bool),
-          nodeptr ↦s[hashtriemap.node :: "isEntry"]□ is_entry ∗
-          if is_entry then
-            ∃ ent,
-              ⌜ent ≠ null⌝ ∗
-              nodeptr ↦s[hashtriemap.node :: "ent"]□ ent ∗
-              nodeptr ↦s[hashtriemap.node :: "ind"]□ null ∗
-              entry γ q ent path
-          else
-            ∃ ind,
-              ⌜length child_path < 16⌝ ∗
-              nodeptr ↦s[hashtriemap.node :: "ent"]□ null ∗
-              nodeptr ↦s[hashtriemap.node :: "ind"]□ ind ∗
-              ▷ child_indirect ind child_path)%I.
-
-  Definition childrenP
-    (child_indirect: loc -d> path -d> iProp Σ)
-    (γ: ghost_names) (q: Qp) (children_slice: slice.t)
-    (children_vals: list atomic.Value.t)
-    (ind: loc) (path: path) : iProp Σ :=
-    "Hchildren" :: [∗ list] i ↦ val ∈ children_vals,
-      let child_path := path ++ [Z.of_nat i] in
-      ∃ (nodeptr: loc),
-        "Hown_child" :: own_Value (slice.elem_ref_f children_slice atomic.Value i) (DfracOwn q)
-          (interface.mk (ptrT.id hashtriemap.node.id) #nodeptr) ∗
-        "Hchild" :: childP child_indirect γ q nodeptr path child_path.
-
-  (* split 50/50 between an invariant and the mutex to allow for lock-free reads *)
-  (* we always have read permission on any indirect, but only can write if we acquire the lock *)
-  (* the only things ever modified are atomic values (atomic pointers), everything else is □ ownership *)
-  Definition indirect_F
-    (γ: ghost_names)
-    (indirect: loc -d> (list Z) -d> iProp Σ)
-    : loc -d> (list Z) -d> iProp Σ :=
-    λ ind path,
-      (∃ (children_vals: list atomic.Value.t) children_slice,
-          "#Hown_children" :: ind ↦s[hashtriemap.indirect :: "children"]□ children_slice ∗
-          "#Hchildren_slice" :: children_slice ↦*□ children_vals ∗
-          "%Hchildren_len" :: ⌜length children_vals = 16%nat⌝ ∗
-          (* "#Hmutex" :: ind ↦s[hashtriemap.indirect :: "mu"]□ mutex ∗ *)
-          "#Hind_inv" :: inv (indN) ((childrenP indirect γ (1/2) children_slice children_vals ind path)) ∗
-          "#Hind_mutex" :: is_Mutex (struct.field_ref_f hashtriemap.indirect "mu" ind) (
-              ∃ (dead: bool),
-                "Hdead" ∷ own_Bool (struct.field_ref_f hashtriemap.indirect "dead" ind) (DfracOwn 1) dead ∗
-                "Hmu_inv" ∷ ((* ⌜¬ dead⌝ -∗  *)childrenP indirect γ (1/2) children_slice children_vals ind path)))%I.
-
-  (* Prove contractiveness *)
-  Global Instance indirect_F_contractive γ : Contractive (indirect_F γ).
+  Lemma map_state_update {γ path hm user_map user_map2 f} key value :
+    let h  := uint.Z (hash_key key) in
+    let f' := (λ h', if decide (h' = h) then <[key:=value]>(f h) else f h') in
+    let um' := <[key:=value]> user_map in
+    let hm' := <[h := (<[key:=value]>) (f h)]> hm in
+    belongs_to_path path h →
+    "Hmap" ∷ map_state γ user_map hm ∗
+    "Huser_map2" ∷ own_ht_map γ user_map2 ∗
+    "Hpath" ∷ own_path γ.(map_name) 1 path f ==∗
+    "Hmap" ∷ map_state γ um' hm' ∗
+    "Huser_map2" ∷ own_ht_map γ um' ∗
+    "Hpath" ∷ own_path γ.(map_name) 1 path f'.
   Proof.
-    rewrite /indirect_F.
-    intros n f g Hfg ind path.
-    f_equiv.
-    f_equiv.
-    f_equiv.
-    f_equiv.
-    have H : ((childrenP f γ (1 / 2) a0 a ind path) ≡{n}≡ (childrenP g γ (1 / 2) a0 a ind path)).
-    { unfold childrenP. repeat f_equiv. unfold childP. solve_contractive. }
-    repeat f_equiv; exact H.
-  Qed.
+    intros.
+    rename H into Hbelongs.
+    iIntros "Hx".
+    iNamed "Hx".
+    iNamed "Hmap".
 
-  Definition indirect (γ: ghost_names) (ind: loc) (path: path) : iProp Σ :=
-    fixpoint (indirect_F γ) ind path.
+    have Hdom : h ∈ path_to_domain path by apply (in_domain _ (hash_key key)).
+    iDestruct (own_path_lookup h _ _ _ _ Hdom with "Hpath") as "[Hptsto Hptsto_close]".
+    iDestruct (map_valid with "Hauth_map Hptsto") as %Hlookup.
+    iDestruct ("Hptsto_close" with "Hptsto") as "Hpath".
 
-  Lemma indirect_unfold γ ind path :
-    indirect γ ind path ⊣⊢
-    indirect_F γ (indirect γ) ind path.
-  Proof. apply (fixpoint_unfold (indirect_F γ)). Qed.
+    iMod (ghost_var_update_halves (<[key:=value]> user_map) with "Huser_map Huser_map2") as "[Huser_map Huser_map2]".
+    iMod (own_path_update_key key value _ _ _ _ Hbelongs with "Hauth_map Hpath") as "(Hauth_map & Hpath)".
+    subst h.
+    set (h := uint.Z (hash_key key)) in *.
+    iNamed.
 
-  #[global] Instance indirect_persistent γ ind path : Persistent (indirect γ ind path).
-  Proof.
-    rewrite indirect_unfold /indirect_F.
-    apply _.
-  Qed.
+    iEval (rewrite decide_True) in "Hctx".
+    set (old := f h) in *.
 
-  Definition ht_inv (ht: loc) (γ: ghost_names) : iProp Σ :=
-    ∃ (rooti: loc) (hm: hash_map) (user_map: gmap K V),
-      "Hauth_map" :: map_ctx γ.(map_name) 1 hm ∗
-      "Huser_map" :: ghost_var γ.(user_name) (DfracOwn (1/2)) user_map ∗
-      "Hown_root" :: own_Value (struct.field_ref_f hashtriemap.HashTrieMap "root" ht) (DfracOwn 1)
-        (interface.mk (ptrT.id hashtriemap.indirect.id) #rooti) ∗
-      "#Hroot_indirect" :: indirect γ rooti [] ∗
-      "%Hflat" :: ⌜user_map = flatten hm⌝ ∗
-      (* bucket correctness - if a key exists, then its in the correct bucket *)
-      "%Hbuckets" :: (⌜∀ h sub k, hm !! h = Some sub →
-                                 uint.Z (hash_key k) = h →
-                                 flatten hm !! k = sub !! k⌝) ∗
-      "%Hbuckets_rev" ∷ (⌜∀ h sub k v,
-                           hm !! h = Some sub →
-                           sub !! k = Some v →
-                           uint.Z (hash_key k) = h⌝).
+    (* have Hhm' : hm' = (<[h := <[key:=value]> old]> hm). *)
+    (* { *)
+    (*   apply map_eq; intro h'. *)
+    (*   destruct (decide (h' = h)) as [->|Hneq]. *)
+    (*   - rewrite lookup_insert. rewrite decide_True; [|reflexivity]. *)
+    (*     rewrite lookup_insert. rewrite decide_True; [|reflexivity]. *)
+    (*     subst f'. *)
+    (*     simpl. *)
+    (*     rewrite decide_True; [|reflexivity]. *)
+    (*     reflexivity. *)
+    (*   - rewrite lookup_insert_ne; [|done]. *)
+    (*     rewrite lookup_insert_ne; [|done]. *)
+    (*     reflexivity. *)
+    (* } *)
 
-  (* Public predicate exposed to clients. *)
-  (* HOCAP style *)
-  Definition is_hashtriemap
-    (γ: ghost_names) (ht: loc) : iProp Σ :=
-    ∃ (seed: w64),
-      "#His_map" :: inv mapN ("Hinv" :: ht_inv ht γ) ∗
-      "#Hseed" :: ht ↦s[hashtriemap.HashTrieMap :: "seed"]□ seed.
-
-  (* Abstract map state seen by clients. *)
-  Definition own_ht_map (γ: ghost_names) (m: gmap K V) : iProp Σ :=
-    ghost_var γ.(user_name) (DfracOwn (1/2)) m.
-
-  Definition ht_au_mask : coPset :=
-    ⊤ ∖ ↑mapN ∖ ↑indN ∖ ↑entryN.
-
-  (* (* Atomic update over the abstract map state. *) *)
-  (* Definition ht_au *)
-  (*   (γ: ghost_names) *)
-  (*   (Φ: gmap K V → iProp Σ) : iProp Σ := *)
-  (*   (|={ht_au_mask, ∅}=> ∃ m, own_ht_map γ m ∗ *)
-  (*                             (own_ht_map γ m ={∅, ht_au_mask}=∗ Φ m))%I. *)
-
-  (* (* AU variant for specs that return a value. *) *)
-  (* Definition ht_au_val *)
-  (*   (γ: ghost_names) *)
-  (*   (Φ: gmap K V → val → iProp Σ) : iProp Σ := *)
-  (*   ht_au γ (λ m, (∀ v, Φ m v)%I). *)
-
-  (* Helper for Load return values. *)
-  Definition ht_load_ret (m: gmap K V) (key: K) : val :=
-    (#(default (default_val K) (m !! key)), #(bool_decide (is_Some (m !! key))))%V.
-
-  (* (* Atomic update that allows changing the abstract map state. *) *)
-  (* Definition ht_au_upd *)
-  (*   (γ: ghost_names) *)
-  (*   (Ψ: gmap K V → gmap K V → iProp Σ) : iProp Σ := *)
-  (*   (|={ht_au_mask, ∅}=> ∃ m, own_ht_map γ m ∗ *)
-  (*     (∀ m', own_ht_map γ m' ={∅, ht_au_mask}=∗ Ψ m m'))%I. *)
-
-  (* (* Helper for LoadOrStore return value and post-state. *) *)
-  (* Definition ht_load_or_store_ret (m: gmap K V) (key: K) (value: V) : val := *)
-  (*   match m !! key with *)
-  (*   | Some v => (#v, #true)%V *)
-  (*   | None => (#value, #false)%V *)
-  (*   end. *)
-
-  (* Definition ht_load_or_store_next (m: gmap K V) (key: K) (value: V) : gmap K V := *)
-  (*   match m !! key with *)
-  (*   | Some _ => m *)
-  (*   | None => <[key := value]> m *)
-  (*   end. *)
-
-  (* Definition ht_au_load_or_store *)
-  (*   (γ: ghost_names) (key: K) (value: V) (Φ: val → iProp Σ) : iProp Σ := *)
-  (*   ht_au_upd γ (λ m m', *)
-  (*                  ⌜m' = ht_load_or_store_next m key value⌝ ∗ *)
-  (*     Φ (ht_load_or_store_ret m key value))%I. *)
-
-  (* Lemma flatten_lookup_Some hm key v : *)
-  (*   flatten hm !! key = Some v → *)
-  (*   ∃ h sub, hm !! h = Some sub ∧ sub !! key = Some v. *)
-  (* Proof. *)
-  (*   intros Hflat. *)
-  (*   induction hm as [|h sub hm Hnotin IH] using map_ind. *)
-  (*   - exists 0, ∅. *)
-  (*     rewrite /flatten in Hflat; simpl in Hflat. *)
-  (*     rewrite lookup_empty in Hflat; congruence. *)
-  (*   - *)
-  (*     rewrite /flatten map_fold_insert_L in Hflat; auto. *)
-  (*     2: { *)
-  (*       intros. *)
-  (*       auto. *)
-  (*       replace (z1 ∪ (z2 ∪ y)) with (z1 ∪ z2 ∪ y). *)
-  (*       { *)
-  (*         replace (z2 ∪ (z1 ∪ y)) with (z2 ∪ z1 ∪ y). *)
-  (*         { *)
-  (*           replace (z1 ∪ z2) with (z2 ∪ z1). *)
-  (*           { *)
-  (*             reflexivity. *)
-  (*           } *)
-  (*           apply map_union_comm. *)
-  (*           apply map_disjoint_spec; intros k v1 v2 Hk1 Hk2. *)
-  (*           admit. *)
-  (*         } *)
-  (*         symmetry. *)
-  (*         apply map_union_assoc. *)
-  (*       } *)
-  (*       symmetry. *)
-  (*       apply map_union_assoc. *)
-  (*     } *)
-  (*     (* now Hflat : (sub ∪ flatten hm) !! key = Some v *) *)
-  (* Admitted. *)
-
-  (* designed to be split between an invariant and a mutex, so that reading can be done outside of the critical section and writing can only be done inside *)
-  Definition init_tok `{!ghost_varG Σ bool} (γ: ghost_names) (b: bool) : iProp Σ :=
-    ghost_var γ.(init_name) (DfracOwn (1/2)) b.
-
-  Definition init_status_done
-    (γ: ghost_names) (ht: loc) (b: bool) : iProp Σ :=
-    (if b then is_hashtriemap γ ht else True%I).
-
-  Definition init_status_inv
-    `{!ghost_varG Σ bool}
-    (ht: loc) (γ: ghost_names) : iProp Σ :=
-    ∃ (b: bool),
-      own_Uint32 (struct.field_ref_f hashtriemap.HashTrieMap "inited" ht) 1
-        (if b then W32 1 else W32 0) ∗
-      init_tok γ b ∗
-      □ init_status_done γ ht b.
-
-  Definition init_status
-    `{!ghost_varG Σ bool}
-    (ht: loc) (γ: ghost_names) : iProp Σ :=
-    inv init_statusN (init_status_inv ht γ).
-
-  (* Initialization lock invariant for HashTrieMap. *)
-  Definition init_mu_inv `{!ghost_varG Σ bool}
-    (ht: loc) (γ: ghost_names) : iProp Σ :=
-    ∃ (b: bool),
-      if b
-      then init_tok γ true
-      else (init_tok γ false ∗
-            (∃ (seed: w64),
-                ht ↦s[hashtriemap.HashTrieMap :: "seed"] seed) ∗
-            own_Value (struct.field_ref_f hashtriemap.HashTrieMap "root" ht) 1 interface.nil
-           )%I.
-
-  Definition init_mu `{!ghost_varG Σ bool}
-    (ht: loc) (γ: ghost_names) : iProp Σ :=
-    is_Mutex (struct.field_ref_f hashtriemap.HashTrieMap "initMu" ht)
-      (init_mu_inv ht γ).
-
-  Definition hashtriemap_init
-    `{!ghost_varG Σ bool}
-    (ht: loc) (γ: ghost_names) : iProp Σ :=
-    "#Hinit" :: init_status ht γ ∗
-    "#Hinit_mu" :: init_mu ht γ.
-
-  Lemma hashtriemap_pre_auth_init
-    `{!mapG Σ w64 w64, !ghost_varG Σ (gmap w64 w64), !ghost_varG Σ bool} :
-    ⊢ |==> ∃ γ,
-      init_tok γ false ∗ init_tok γ false.
-  Proof.
-    iMod (ghost_var_alloc (false)) as (init_γ) "[Hinit1 Hinit2]".
-    iMod (ghost_var_alloc (∅ : gmap K V)) as (map_γ) "Hmap".
-    iMod (ghost_var_alloc (∅ : gmap K V)) as (user_γ) "[Huser1 Huser2]".
-    iModIntro.
-    iExists (mkNames map_γ init_γ user_γ).
+    (* iEval (rewrite -Hhm') in "Hctx". *)
     iFrame.
-  Qed.
 
-  Lemma hashtriemap_zero_init
-    `{!mapG Σ Z (gmap K V), !mapG Σ K V, !ghost_varG Σ (gmap w64 w64), !ghost_varG Σ bool}
-    (ht: loc) E (P: gmap w64 w64 → iProp Σ) :
-    ht ↦ default_val hashtriemap.HashTrieMap.t ={E}=∗
-    ∃ γ, hashtriemap_init ht γ.
-  Proof.
-    iIntros "Hht".
-    iDestruct (struct_fields_split with "Hht") as "Hfields".
-    iNamed "Hfields".
-    simpl.
-    iMod (hashtriemap_pre_auth_init) as (γ) "(Htok1 & Htok2)".
+    iPureIntro.
 
-    iApply struct_fields_split in "Hinited".
-    iNamed "Hinited".
-    iDestruct (Uint32_unfold with "Hv") as "Hinited".
-    iClear "H_0".
+    (* clear Hhm'. *)
 
-    iApply struct_fields_split in "Hroot".
-    iNamed "Hroot".
-    simpl.
-    iDestruct (Value_unfold with "Hv") as "Hroot".
-
-    iMod (inv_alloc init_statusN _ (init_status_inv ht γ) with "[Htok1 Hinited]") as "#Hinit".
+    assert (Hum' : (um' = flatten hm')).
     {
-      iNext.
-      iExists false.
-      iFrame.
-      done.
-    }
-    set (m := struct.field_ref_f hashtriemap.HashTrieMap "initMu" ht).
-
-    iMod (init_Mutex (init_mu_inv ht γ) E m with "HinitMu [Htok2 Hseed Hroot]") as "Hmutex".
-    {
-      iNext.
-      iExists false.
-      iFrame.
+      subst f'.
+      subst um' hm'.
+      symmetry.
+      subst user_map.
+      (* rewrite decide_True; [|reflexivity]. *)
+      apply (flatten_update_update hm h key value old).
+      - exact Hlookup.
+      - reflexivity.
+      - intros.
+        eapply Hbuckets_rev.
+        + exact H.
+        + exact H0.
     }
 
-    iModIntro.
-    iExists γ.
-    iFrame.
-    iFrame "#".
+    split; [exact Hum'|].
+    split.
+    {
+      intros h0 sub k Hhm' Hhash.
+      rewrite -Hum'.
+      subst um' hm'.
+      subst f'.
+      destruct (decide (h0 = h)) as [->|Hneq].
+      - rewrite lookup_insert in Hhm'.
+        rewrite decide_True in Hhm'; [|reflexivity].
+        (* rewrite decide_True in Hhm'; [|reflexivity]. *)
+        inversion Hhm'; subst sub; clear Hhm'.
+        destruct (decide (k = key)) as [->|Hk].
+        + rewrite lookup_insert. rewrite lookup_insert.
+          rewrite decide_True; [|reflexivity].
+          rewrite decide_True; [|reflexivity].
+          done.
+        + rewrite lookup_insert_ne; [|done].
+          have Hnone_k : user_map !! k = old !! k.
+          {
+            rewrite Hflat.
+            apply (Hbuckets h); auto.
+          }
+          rewrite Hnone_k.
+          rewrite lookup_insert_ne; [|done].
+          done.
+      - rewrite lookup_insert_ne in Hhm'; [|done].
+        destruct (decide (k = key)) as [->|Hk].
+        + exfalso. apply Hneq.
+          subst h. rewrite Hhash.
+          done.
+        + rewrite lookup_insert_ne; [|done].
+          rewrite Hflat.
+          eapply Hbuckets; eauto.
+    }
+    {
+      subst f'.
+      subst hm'.
+      simpl in *.
+      (* rewrite decide_True in Hum'; [|reflexivity]. *)
+      (* rewrite decide_True; [|reflexivity]. *)
+      intros.
+      destruct (decide (h0 = h)) as [->|Hneq].
+      - rewrite lookup_insert in H.
+        rewrite decide_True in H; [|done].
+        inversion H; subst sub; clear H.
+        destruct (decide (k = key)) as [->|Hk].
+        + done.
+        + rewrite lookup_insert_ne in H0; [|done].
+          apply (Hbuckets_rev h old k v); auto.
+      - rewrite lookup_insert_ne in H; [|done].
+        eapply Hbuckets_rev; eauto.
+    }
   Qed.
 
 End model.
